@prefix owl: <http://www.w3.org/2002/07/owl#> .
@prefix rdfs: <http://www.w3.org/2000/01/rdf-schema#> .
@prefix rdf: <http://www.w3.org/1999/02/22-rdf-syntax-ns#> .
@prefix xsd: <http://www.w3.org/2001/XMLSchema#> .
@prefix vann: <http://purl.org/vocab/vann/> .
@prefix dc: <http://purl.org/dc/elements/1.1/> .
@prefix vir: <http://w3id.org/vir#> . 
@prefix crm: <http://www.cidoc-crm.org/cidoc-crm/> . 
@prefix mimatex: <https://github.com/ValentinaPasqual/mima/edit/master/mima-tex.ttl#> . 

<https://github.com/ValentinaPasqual/mima/edit/master/mima-tex.ttl#> 
                        rdf:type owl:Ontology ;
                        dc:creator "Valentina Pasqual" ;
                        dc:date "2020-02-14" ;
                        dc:description ""@en ;
                        dc:title "CRMTex RDF VERSION for testing data mima - Multi-Interpretation model on Manuscript visual Apparatus"@en ;
                        vann:preferredNamespacePrefix "mimatex" ;
                        vann:preferredNamespaceUri "https://github.com/ValentinaPasqual/mima/edit/master/mima_ontology.ttl#" ;
                        owl:versionInfo "1.0" .


########################################################################################################################
#################################################### CLASSES ###########################################################
########################################################################################################################

mimatex:TX1_Written_Text a owl:Class ; 
    rdfs:subClassOf crm:E25_Man-Made_Feature ;
    rdfs:comment """Subclass of TX1 Written Text intended to identify portions of text considered to be
of particular significance by scholars, as witnesses of a certain meaning or bearers of
a particular phenomenon relevant to the investigation, study and understanding of the
ancient text. Examples of such text portions are: columns, fragments, sections,
paragraphs, as well as single words or letters, or other components of the written text.
To each of these entities can be associated a single production event (TX2) or
destruction event (E6), as in the case of letters or words damaged or worn by
atmospheric agents or human interventions, as well as specific conditions (E3) for
documenting its status during the observation process (S4). The relationship between
a written text (TX1) and its components is documented through the TXP4 is
constituted by property."""@en ;
    rdfs:label "Written Text" .

mimatex:TX7_Written_Text_Fragment a owl:Class ; 
    rdfs:subClassOf mimatex:TX1_Written_Text ;
    rdfs:comment """Subclass of E25 Man-Made Feature intended to describe a particular feature (i.e., set
of glyphs) created (i.e., written) on various kinds of support, having semiotic
significance and the declared purpose of conveying a specific message towards a
given recipient or group of recipients."""@en ;
    rdfs:label "Written Text Fragment" .

mimatex:TX2_Writing a owl:Class ;
    rdfs:subClassOf crm:E12_Production ;
    rdfs:comment """Subclass of E12 Production indicating the activity of creating textual entities using
various techniques (painting, sculpture, etc.) and by means of specific tools on a
given physical carrier in a non-mechanical way."""@en ;
    rdfs:label "Writing" .

mimatex:TX3_Writing_System a owl:Class ;
    rdfs:subClassOf crm:E29_Design_or_Procedure ;
    rdfs:comment """Subclass of E29 Design or Procedure refers to a conventional system consisting of a
set of signs (graphemes, E90) used to codify a natural language. A writing system
can be used to notate different natural languages, by means of specific rules in the
combination and phonological value assignment of the chosen graphemes. It is used
to produce a TX1 Written Text during a TX2 Writing event."""@en ;
    rdfs:label "Writing System" .


########################################################################################################################
############################################## OBJECT PROPERTIES #######################################################
########################################################################################################################

mimatex:TXP1_used_writing_system a owl:ObjectProperty ;
    rdfs:domain mimatex:TX2_Writing ;
    rdfs:comment """This property is intended to identify the specific instance of TX3 Writing System
employed during the writing event that led to the creation of a TX1 Written Text."""@en ;
    rdfs:label "used writing system" ;
    rdfs:range mimatex:TX3_Writing_System ;
    owl:inverseOf mimatex:TXP1_writing_system_used_for . 
